New findings/ideas work very well. No need for parametricity

io/Poly.fst
@@ -26,8 +26,8 @@ type int1 : Type u#1 = Universe.raise_t int
 type src_ctx1 = ((int1 -> free.m int1) -> free.m int1) -> free.m (int1 -> free.m int1)
 type tgt_ctx1 = mon:monad -> acts mon -> ((int1 -> mon.m int1) -> mon.m int1) -> mon.m (int1 -> mon.m int1)
 
-val backtranslate : tgt_ctx1 -> src_ctx1
-let backtranslate (tgt_ctx:tgt_ctx1) (pprog_cb:((int1 -> free.m int1) -> free.m int1)) : free.m (int1 -> free.m int1) = 
+val backtranslate1 : tgt_ctx1 -> src_ctx1
+let backtranslate1 (tgt_ctx:tgt_ctx1) (pprog_cb:((int1 -> free.m int1) -> free.m int1)) : free.m (int1 -> free.m int1) = 
   let src_ctx : ((int1 -> free.m int1) -> free.m int1) -> free.m (int1 -> free.m int1) = tgt_ctx free free_acts in
   let r : free.m (int1 -> free.m int1) = src_ctx pprog_cb in 
   r
@@ -35,102 +35,63 @@ let backtranslate (tgt_ctx:tgt_ctx1) (pprog_cb:((int1 -> free.m int1) -> free.m 
 let src_prog1 : Type = src_ctx1 -> free.m int1
 let tgt_prog1 : Type = tgt_ctx1 -> free.m int1
 
-val compile : src_prog1 -> tgt_prog1
-let compile src_prog tgt_ctx : free.m int1 = 
-  src_prog (backtranslate tgt_ctx)
+val compile1 : src_prog1 -> tgt_prog1
+let compile1 src_prog tgt_ctx : free.m int1 = 
+  src_prog (backtranslate1 tgt_ctx)
 
 (* Conclusion until now, it is that we do not need to do 
    recursively compile/instrument things. It is enough to
    have the context as an effectful polymorphic type and 
    instantiate with free and the actions **)
 
-(* Problem to solve: how to derive the type of the program in the target from the type in the source
-   Two initial ideas: 
-   1. have something that gives us the type in the source and the target (Kleisli/Code)
-   2. use TypeClasses.*)
-
-(* Next challenge is to have Dijkstra Monads at all positions, instead of the free monad. 
-   My intuition says we should get this from parametricity. *)
+(** *** Try new idea **)
 assume type w (a:Type)
 assume val theta : (#a:Type) -> (c:free.m a) -> w a
 assume val w_ord : w 'a -> (w 'a) -> Type0
 
-type dm a (wp:w a) = c:(free.m a){wp `w_ord` theta c} 
-
 assume type pi_type
 assume val pi_as_w : (#a:Type) -> pi_type -> w a
 
-(** *** Parametricity **)
-noeq
-type monad_p (mon:monad) = {
-  m_p : a:Type -> a_p:(a -> Type) -> x:(mon.m a) -> Type;
-  ret_p : a:Type -> a_p:(a -> Type) -> (x:a) -> x_p:(a_p x) -> Lemma (m_p a a_p (mon.ret x));
+type dm (pi:pi_type) (a:Type) = c:(free.m a){pi_as_w pi `w_ord` theta c} 
+
+(* this is easy to prove since ret produces the empty trace *)
+assume val lemma_return_dm (pi:pi_type) (x:'a) :
+  Lemma (pi_as_w pi `w_ord` theta (free.ret x))
+
+(* this is also easy to prove based on how enforced_locally is defined *)
+assume val lemma_bind_dm (pi:pi_type) (m:dm pi 'a) (k:'a -> dm pi 'b) :
+  Lemma (pi_as_w pi `w_ord` theta (free.bind m k))
+
+let dm_mon (pi:pi_type) : monad = {
+  m = dm pi;
+  ret = (fun (x:'a) -> 
+    lemma_return_dm pi x;
+    free.ret x);
+  bind = (fun (m:dm pi 'a) (k:'a -> dm pi 'b) -> 
+    lemma_bind_dm pi m k;
+    free.bind m k)
 }
 
-[@@ "opaque_to_smt"]
-type io_cmds_p (cmd:io_ops) = True
+assume val dm_acts (pi:pi_type) : acts (dm_mon pi)
 
-[@@ "opaque_to_smt"]
-type io_sig_args_p (op:io_ops) (arg:io_sig.args op) = True
+assume type ct (m:Type u#a -> Type u#(max 1 a))
 
-[@@ "opaque_to_smt"]
-type io_sig_res_p (op:io_ops) (arg:io_sig.args op) (res:io_sig.res op arg) = True
+type src_ctx2 (pi:pi_type) = ct u#a (dm_mon pi).m
+type tgt_ctx2 = mon:monad -> acts mon -> ct mon.m
 
-type acts_p (mon:monad) (mon_p:monad_p mon) (theActs:acts mon) = 
-  op:io_ops -> op_p : (io_cmds_p op) -> 
-  arg:io_sig.args op -> arg_p : (io_sig_args_p op arg) ->
-  Lemma (mon_p.m_p (io_sig.res op arg) (io_sig_res_p op arg) (theActs op arg))
+(* TODO: looks like tgt_ctx and src_ctx must be in the same universe *)
+val backtranslate2 : pi:pi_type -> tgt_ctx2 u#a u#b -> src_ctx2 u#a pi
+let backtranslate2 pi tgt_ctx : src_ctx2 pi =
+  tgt_ctx (dm_mon pi) (dm_acts pi)
 
+let src_prog2 (ipi:pi_type) (vpi:pi_type) : Type = src_ctx2 u#a ipi -> (dm_mon vpi).m int1
+let tgt_prog2 : Type = tgt_ctx2 -> free.m int1
 
-(** **** Parametricity - instances **)
-let free_p (pi:pi_type) : monad_p free = {
-  m_p = (fun a a_p tree -> pi_as_w pi `w_ord` theta tree);
-  ret_p = (fun a a_p tree tree_p -> (* This was unit before *) admit ());
-}
+val compile2 : (#ipi:pi_type) -> (#vpi:pi_type) -> src_prog2 u#a ipi vpi -> tgt_prog2 u#a u#b 
+let compile2 #ipi src_prog tgt_ctx : free.m int1 = 
+  src_prog (backtranslate2 ipi tgt_ctx)
 
-assume val wrap : pi_type -> acts free -> acts free
-
-val wrap_p : (pi:pi_type) -> (ca:(acts free)) -> acts_p free (free_p pi) (wrap pi ca)
-let wrap_p pi ca (op:io_ops) op_p (arg:io_sig.args op) arg_p : 
-  Lemma ((free_p pi).m_p (io_sig.res op arg) (io_sig_res_p op arg) ((wrap pi ca) op arg)) = 
-  (* this was proved before *)
-  admit ()
-
-type ct_p 
-  (mon:monad) (mon_p:monad_p mon)
-  (a b:Type)
-  (c:a -> mon.m b) =
-  squash (forall x. mon_p.m_p b (fun x -> True) (c x))
-
-type ctx_p 
-  (mon:monad) (mon_p:monad_p mon) 
-  (theActs:acts mon) (theActs_p:acts_p mon mon_p theActs)
-  (a:Type)
-  (b:Type) 
-  (c:(mon:monad -> acts mon -> a -> mon.m b)) =
-  ct_p mon mon_p a b (c mon theActs)
-
-assume val ctx_param : 
-  (mon:monad) -> (mon_p:monad_p mon) ->
-  (theActs:acts mon) -> (theActs_p:acts_p mon mon_p theActs) ->
-  (a:Type) ->
-  (b:Type) ->
-  (c:(mon:monad -> acts mon -> a -> mon.m b)) ->
-  Lemma (ctx_p mon mon_p theActs theActs_p a b c)
-
-open FStar.Tactics
-
-val cast_to_dm_iio  : 
-  (#a:Type) -> 
-  (#b:Type) -> 
-  ipi:pi_type ->
-  (mon:monad -> acts mon -> a -> mon.m b) ->
-  (x:a -> dm b (pi_as_w ipi))
-let cast_to_dm_iio #a #b ipi c x : _ by (norm [delta_only [`%Mkmonad_p?.m_p;`%free_p]]; norm [iota]; explode ()) =
-  let c' : a -> free.m b = c free (wrap ipi free_acts) in
-  let tree : free.m _ = c' x in
-  ctx_param free (free_p ipi) (wrap ipi free_acts) (wrap_p ipi free_acts) a b c;
-  assert (pi_as_w ipi `w_ord` theta tree);
-  tree
-
-
+(* Problem to solve: how to derive the type of the program in the target from the type in the source
+   Two initial ideas: 
+   1. have something that gives us the type in the source and the target (Kleisli/Code)
+   2. use TypeClasses.*)
